.

theories/Prelude/PreludeUtil.v
@@ -550,6 +550,33 @@ Module MyData.
     end.
   Proof. destruct i; reflexivity. Qed.
 
+  Lemma evalFin_inj {n : nat} (i1 : Fin n) (i2 : Fin n)
+    (hyp_eq : evalFin i1 = evalFin i2)
+    : i1 = i2.
+  Proof.
+    unfold evalFin in hyp_eq.
+    rewrite <- getFin_runFin_id with (i := i1).
+    rewrite <- getFin_runFin_id with (i := i2).
+    destruct (runFin i1) as [m1 hyp_lt1].
+    destruct (runFin i2) as [m2 hyp_lt2].
+    cbn in *. subst m1. eapply eq_congruence, le_pirrel.
+  Qed.
+
+  Definition incrFin {m : nat} : forall n : nat, Fin m -> Fin (n + m) :=
+    fix incrFin_fix (n : nat) (i : Fin m) {struct n} : Fin (n + m) :=
+    match n as x return Fin (x + m) with
+    | O => i
+    | S n' => FS (incrFin_fix n' i)
+    end
+  .
+
+  Lemma incrFin_spec {m : nat} (n : nat) (i : Fin m)
+    : evalFin (incrFin n i) = n + evalFin i.
+  Proof with eauto.
+    induction n as [ | n IH]; simpl...
+    rewrite evalFin_unfold. eapply eq_congruence...
+  Qed.
+
   Inductive vector (A : Hask.t) : nat -> Hask.t :=
   | VNil : vector A (O)
   | VCons (n : nat) (x : A) (xs : vector A n) : vector A (S n)
